examples/compilation/to_word/word_cse_testScript.sml
@@ -17,15 +17,38 @@ End
 val tm' = “let p = word_cse_compact ^tm in
            remove_dead p LN”
 
-val prog = “(Seq (Inst (Arith (Binop Add 3 1 (Reg 2)))) (Inst (Arith (Binop Add 4 1 (Reg 2)))))”
+val prog = “Seq (Inst (Const 1 0w)) (Inst (Const 3 5w))”
 
-val prog2 = “Seq (Move 0 [(37,2);(39,4)]) (If Equal 41 (Imm 2w) (Return 37 2) (Return 37 2))”;
+val prog = “Seq (Inst (Const 1 0w))
+             (Seq (Inst (Arith (Binop Add 3 1 (Reg 1))))
+              (Inst (Arith (Binop Add 4 1 (Reg 1)))))”
 
+val prog2 = “(Seq (Move 0 [(37,2);(39,4)]) (If Equal 41 (Imm 2w) (Return 37 2) (Return 37 2))):64 wordLang$prog”;
 
-EVAL “^tm”;
+val fact_begin = “Move 1 [(37,0); (41,2); (45,4); (49,6)] ▸
+                  Inst (Const 189 0w) ▸ Inst (Const 193 0w) ▸
+                  OpCurrHeap Add 69 37 ▸
+                  OpCurrHeap Add 71 37 ▸
+                  Inst (Arith (Shift Lsr 65 41 9)) ▸
+                  Inst (Arith (Shift Lsr 67 41 9))
+                 ” (*works *)
 
-EVAL “word_cse_compact ^prog2”;
+val fact_begin2 = “Move 1 [(37,0); (41,2); (45,4); (49,6)] ▸
+                   Inst (Const 53 18w) ▸ Move 0 [(2,45)] ▸
+                   Move 1 [(181,37); (177,49)] ▸ Inst (Const 185 0w) ▸
+                   Inst (Const 189 0w) ▸ Inst (Const 193 0w) ▸ Move 1 [(197,53)] ▸
+                   Inst (Const 201 0w) ▸ Move 1 [(205,41)] ▸ Move 1 [(209,45)] ▸
+                   Inst (Const 213 0w) ▸ Inst (Const 217 0w)
+                   ”
 
+EVAL “^tm'”;
+
+EVAL “word_cse_compact ^prog”;
+
+     EVAL “w2n 5w = w2n 0w”;
+
+EVAL “word_cse_compact ^fact_begin”;
+EVAL “w2n_def 0w”
 val res = EVAL tm';
 
 val res2 = EVAL “word_cse_compact ^tm”;
